Let $f(x)=t_nx^n+\dotsb+t_0$.  Then
\[ \Disc(f) = \frac{(-1)^{n(n-1)/2}\Res(f,f')}{t_n} \]
This is what we will prove, eventually.
%
\begin{flalign*}
\lem && f(x)&=t_n\prod_{i=1}^n(x-\alpha_i) && \\
&& g(x)&=u_m\prod_{i=1}^m(x-\beta_i) && 
\end{flalign*}
Then $\Res(f,g)=t_n^m u_m^n \prod_{i,j}(\alpha_i-\beta_j)$

\textbf{Proof of lemma: }We showed $\Res(f,g)=t_n^mu_m^n(\text{symmetric polynomial in $\alpha_i$, $\beta_j$})$ by showing that
\begin{align*}
\phi(x) &= T_n \prod(x-a_i) \\
\psi(x) &= U_m \prod(x-b_i)
\end{align*}
satisfy $\Res(\phi,\psi)=T_n^mU_m^n\cdot(\text{some polynomial symmetric in $a_i$ and $b_j$})$

Next, we will show that $\Res(f,g)=0$ \emph{iff} $\gcd(f,g)\neq1$.  To see this, note that $\gcd(f,g)\neq1$ \emph{iff} there are polynomials $p(x)$, $q(x)$ of degrees at most $m-1$, $n-1$, respectively, such that $fp=gq$.

This is equivalent to saying that $\brace{f,xf,\dotsc,x^{m-1}f,g,xg,\dotsc,x^{n-1}g}$ is linearly dependent.  Writing this out in terms of the basis $\brace{1,x,\dotsc,x^{n+m-1}}$, we see that $\gcd(f,g)\neq1$ \emph{iff}
\[ \det\begin{bmatrix}
t_n & t_{n-1} & \hdotsfor{1} & t_0 \\
& t_n & \hdotsfor{2} & t_0 \\
& & \ddots & & & \ddots \\
& & & t_n & \hdotsfor{2} & t_0 \\
u_m & u_{m-1} & \hdotsfor{2} & u_0 \\
 & \ddots & & & & \ddots \\
 & & u_m & \hdotsfor{3} & u_0
\end{bmatrix}\footnote{$m$ rows, $n$ rows} = 0 = \Res(f,g) \]
Therefore, $\Res(\phi,\psi)=CT_n^mU_m^n\prod_{i,j}(a_i-b_j)$ for some $C\in F$.

To find $C$, compute $\Res(x^n, x^m-1)$.
\[ = \det\begin{bmatrix}
1 \\
& \ddots \\
& & 1 \\
1 & & & -1 \\
& \ddots & & & \ddots \\
& & 1 & \hdotsfor{2} & -1
\end{bmatrix}\footnote{$m$ rows, $n$ rows} = (-1)^n \]
\begin{align*}
\Res(x^n, x^m-1) &= C\prod_{i=1}^n\prod_{j=1}^m(0-\beta_j) \\
&= C\prod_{j=1}^m (-\beta_j)^n \\
&= C(-1)^{mn}\paren[\Big]{\prod_{j=1}^m\beta_j}^n \\
&= C(-1)^{mn}\paren[\big]{(-1)^{m+1}}^n \\
&= C(-1)^n
\end{align*}
$\implies C=1$ \qed\ lemma

$g(\alpha_i)=u_m\prod_j(\alpha_i-\beta_j)$
\begin{align*}
\implies\Res(f,g) &= t_n^m\prod_{i=1}^n g(\alpha_i) \\
&= (-1)^{nm} u_m^n \prod_{j=1}^m f(\beta_j)
\end{align*}
Now, $\Disc(f)=t_n^{2n-2}\prod_{i<j}(\alpha_i-\alpha_j)^2$, and $f'(\alpha_i)=\left.\frac{\d}{\d x}\right\rvert_{x=\alpha_i} t_n \prod_{j=1}^n(x-\alpha_j)=\prod_{j\neq i}(\alpha_i-\alpha_j)$.
\begin{align*}
\text{So } \frac{\Res(f,f')}{t_n} &= t_n^{n-2}\prod_{i=1}^n f'(\alpha_i) \\
&= t_n^{n-2}t_n^n \prod_{i=1}^n\prod_{j\neq i}(\alpha_i-\alpha_j) \\
&= (-1)^{n(n-1)/2}\footnote{one factor of $-1$ for each pair $(i,j)$, $i\neq j$}t_n^{2n-2}\prod_{i<j}(\alpha_i-\alpha_j)^2 \\
&= (-1)^{n(n-1)/2}\Disc(f,f')
\end{align*}
This proves the claim!

\eg $f(x)=x^2+bx+c$
\begin{gather*}
\implies \Disc(f) = -\Res(f,f') \\
= - \Res(x^2+bx+c,2x+b) \\
= - \det\begin{bmatrix}
1 & b & c \\
2 & b & 0 \\
0 & 2 & b
\end{bmatrix} \\
= -(b^2+4c-2b^2) = b^2 - 4c
\end{gather*}
This looks familiar:
\[ x = \frac{-b\pm\sqrt{b^2-4c}}{2} \]
