\textbf{Addendum to \S9: Fields} \\
\textbf{Notation: }$\alpha\colon R\to R'$ isomorphism of rings induces an isomorphism
\begin{align*}
\alpha\colon &R[x] \to R'[x] \\
&a_0+\dotsb+a_nx^n\mapsto\alpha(a_0)+\alpha(a_1)x+\dotsb+\alpha(a_n)x^n
\end{align*}
\lem $\alpha\colon F\to F'$ isomorphism of fields, \\
two simple algebraic extensions
\[ \xymatrix{
F(a) \ar@{-}[d]\ar@{.>}[r]^\beta & F'(b) \ar@{-}[d] \\ %dotted arrow
F \ar[r]^\alpha_\cong & F'
} \]
with $f=\text{minimal polynomial of $a$ over $F$}\in F[x]$, such that \\ $\alpha(f)=\text{minimal polynomial of $b$ over $F'$}\in F'[x]$. \\
(i.e., $\alpha$ takes minimal polynomial of $a/F$ to minimal polynomial of $b/F'$) \\
\emph{Then}, $\alpha$ extends to an isomorphism
\[ \beta\colon F(a) \to F'(b) \]
with $\beta(a)=b$. \\
That is:
\begin{itemize}
\item $\beta|_F = \alpha$
\item $\beta(a) = b$
\end{itemize}
\ex converse is also true \\
\pf Let $f'=\alpha(f)=\text{minimal polynomial of $b$ over $F'$}$
%\[ \xymatrix{
%F[x] \ar@{-}[d]\ar[r]^\alpha_\cong F'[x] \ar@{-}[d] \ar@{>>}[r]^\pi F'[x]/(f') %\ar[r]^\cong_\rho F'(b) \\
%F \ar[r]^\alpha_\cong & F'
%} \]
%\[ \left. \begin{aligned}
%\rho \circ \pi \circ \alpha(h) &= 0 \\
%\iff \pi\circ\alpha(h) &= 0 \\
%\iff \alpha(h) &\in (f')
%\end{aligned} \right\} \ker(\alpha\circ\pi\circ\rho) = \alpha^{-1}(f'\cdot F'[x]) %=\footnote{the $\alpha(f)=f'$} f\cdot F[x] = (f) \]
\[ \xymatrix{
F[x] \ar@{-}[d]\ar[r]^\alpha_\cong & F'[x] \ar@{-}[d] \\
F \ar[r]^\alpha_\cong & F'
} \]
$\alpha$ is an isomorphism
\[ \alpha^{-1}(f'\cdot F'[x]) = f\cdot F[x] \]
Then $\alpha$ induces
\begin{align*}
\overline\alpha\colon &f[x]/(f) \overset{\cong}{\to} F'[x]/(f') \\
&h+(f) \mapsto \alpha(h)+(f')
\end{align*}
check that $\overline\alpha$ is indeed an isomorphism.
\[ \xymatrix{
F(a) \ar@{<}`u[r]`[rrr]^\beta[rrr] & \ar[l]^\phi_\cong F[x]/(f) \ar[r]^\cong_{\overline\alpha} & F'[x]/(f') \ar[r]_{\phi'}^\cong & F'(b) \\
h(a) & \ar@{|->}[l] h + (f) & h'+(f') \ar@{|->}[r] & h'(b)
} \]% line from F(a) to F'(b) overset \beta
\[ \beta \coloneqq \phi'\circ\overline\alpha\circ\phi^{-1}\colon F(a)\to F'(b) \]
is an isomorphism. \\
Given $c\in F$,
\begin{align*}
\beta(c) &= \phi'\circ\overline\alpha\circ\phi^{-1}(c) \\
&= \phi'\circ\overline\alpha(c+(f)) \\
&= \phi'(\alpha(c)+(f')) \qquad \alpha(c)\in F' \\
&= \alpha(c)
\end{align*}
Therefore $\beta|_F = \alpha$.
\begin{align*}
\beta(a) &= \phi'\circ\overline\alpha\circ\phi^{-1}(a) \\
&=\phi'\circ\overline\alpha(x+(f)) \\
&=\phi'(x+(f')) \\
&=b
\end{align*}
\prop $\alpha\colon F\to F'$ isomorphism \\
$f\in F[x]$, $\deg f>0$. \\
Let $K$ be a splitting field of $f$ over $F$ \\
Let $K'$ be a splitting filed of $\alpha(f)$ over $F'$
\[ \xymatrix{
K \ar@{-}[d]\ar@{.>}[r]^\beta & K' \ar@{-}[d] \\ %dotted arrow
F \ar[r]^\alpha_\cong & F'
} \qquad f'=\alpha(f) \]
Then $\alpha$ extends to an isomorphism $\beta\colon K\to K'$. \\
So $\beta|_F=\alpha$. \\
\remark When $F=F'$ and $\alpha=\id$ this proposition says that any two splitting fields of $f$ over $F$ are \emph{isomorphic over $F$}. \\
That is, $\beta|_F=\id$.
\[ \xymatrix{
K \ar@{.>}[rr] & & K' \\ %dotted
 & \ar@{-}[ul] F \ar@{-}[ur] &
} \]
(\defin $S$ and $S'$ extensions of a ring $R$, are \emph{isomorphic over $R$} if there is an isomorphism $\beta\colon S\to S'$ such that $\beta|_R=\id$.) \\
\pf Induction on $[K:F]=n$. \\
$n=1$: $K=F$ $\implies$ $f$ factors completely into linear factors in $F[x]$ \\
$\implies$ $\alpha(f)$ factors into linear factors in $F'[x]$ \\
$\implies$ $K'=F'$ \\
So $\beta=\alpha$ works. $\checkmark$ \\
$n>1$: $f$ must have an irreducible factor $g\in F[x]$ which is \emph{not} linear. $\implies\deg g>1$ \\
Let $a\in K$ be a root of $g$. \\
(exists since $g\mid f$ and $K=\text{splitting field of $f$ over $F$}$) \\
Let $g'=\alpha(g)\in F'[x]$. \\
So $g'\mid\alpha(f)$ $\implies$ $g'$ has a root $b\in K'$.
\[ \xymatrix{
K \ar@{-}[d] \ar@{.>}[r]^\beta & K' \ar@{-}[d] \\ %dotted
F(a) \ar[r]^\beta\ar@{-}[d]^{\mathllap{\text{minimal polynomial is $g$}\quad}} & F'(b) \ar@{-}[d]_{\mathrlap{\quad\text{minimal polynomial $g'=\alpha(g)$}}} \\
F \ar[r]^\alpha_\cong & F'
} \]
Lemma $\implies$ Can extend $\alpha$ to an isomorphism $\beta\colon F(a)\to F'(b)$ which extends $\alpha$ \\
But $K$ is still the splitting field of $f$ over $F(a)$ \\
And $K'$ is a splitting field of $\alpha(f)$ over $F'(b)$.  Note $\beta(f)=\alpha(f)$
\[ [K:F(a)] = \frac{n}{\deg g} < n \]
By Induction Hypothesis $\beta$ extends to a $\hat\beta\colon K\to K'$.
\[ \hat\beta|_F = \beta|_F = \alpha \]
So $\hat\beta$ works.

\textbf{\S10:} \\
\cor $K,L$ finite fields, $\abs K=\abs L=p^n$. \\
Suppose $K,L$ are both extensions of a finite field $F$.
\[ \xymatrix{
K \ar@{.>}[rr]^\cong \ar@{-}[dr] & & \ar@{-}[dl] L \\ %dotted
 & F \ar@{-}[d] & \\
 & \Z_p &
} \]
Then $K$ and $L$ are isomorphic over $F$. \\
\pf $K$ and $L$ are both splitting fields of $x^{p^n}-x$ over $\Z_p$, hence also over $F$. \\
Apply proposition (in fact the Remark).
